Start of transition to better handling of namespaces.  Name information is now stored in either the "env", or the "genv".  The latter is used for non-automatic names and classes, that are not created dynamically.  The former is used for the rest.  The basic assumption is that processing of external declarations, now to be done in the new theory "name_resolution", will resolve all names as it reads in external declarations.  This will extend to field references, which are allowed to be full-blown ids (not just sfields).  I.e., it's legitimate C++ to write   { C c; c.B::fld = 3; }  believe it or not, and the abstract syntax now reflects this.

holsrcs/class_infoScript.sml
@@ -20,18 +20,25 @@ open statesTheory aggregatesTheory
 val _ = new_theory "class_info";
 
 val is_class_name_def = Define`
-  is_class_name st cppid = cppid IN FDOM st.classmap
+  is_class_name st cppid = if is_abs_id cppid then
+                             is_class_name_env st.genv cppid
+                           else is_class_name_env st.env cppid
 `;
 
+val cinfo0_def = Define`
+  cinfo0 s cnm = (item (THE (elookup_class (if is_abs_id cnm then s.genv
+                                            else s.env)
+                                           cnm))).info
+`
 
 
 val cinfo_def = Define`
-  cinfo s cnm : class_info = FST (THE (s.classmap ' cnm))
+  cinfo s cnm : class_info = FST (THE (cinfo0 s cnm))
 `;
 
 (* set of a state's fully defined class *)
 val defined_classes_def = Define`
-  defined_classes s = FDOM (deNONE s.classmap)
+  defined_classes s = { id | is_class_name s id /\ ~(cinfo0 s id = NONE) }
 `;
 
 (* similarly, direct base classes, in order of declaration *)
@@ -99,7 +106,7 @@ val has_user_constructor_def = Define`
   has_user_constructor s cnm =
     cnm IN defined_classes s /\
     ?ci userdefined.
-       (s.classmap ' cnm = SOME (ci,userdefined)) /\
+       (cinfo0 s cnm = SOME (ci,userdefined)) /\
        (DefaultConstructor IN userdefined \/ CopyConstructor IN userdefined)
 `;
 
@@ -115,18 +122,13 @@ val is_aggregate_def = Define`
   (is_aggregate s _ = F)
 `;
 
-val strip_array_def = Define`
-  (strip_array (Array bt n) = strip_array bt) /\
-  (strip_array t = t)
-`;
-
 (* 9 p4  : POD types *)
 val (PODstruct_rules, PODstruct_ind, PODstruct_cases) = Hol_reln`
   (!s cnm.
      cnm IN defined_classes s /\
      is_aggregate s (Class cnm) /\
      DISJOINT {Destructor; CopyAssignment}
-              (SND (THE (s.classmap ' cnm))) /\
+              (SND (THE (cinfo0 s cnm))) /\
      (!fldname fldty prot.
          MEM (FldDecl fldname fldty, F, prot)
              ((cinfo s cnm).fields) ==>
@@ -295,7 +297,7 @@ val MethodDefs_def = Define`
                            (cinfo s (LAST Cs)).fields }
 `
 
-(* s |- C has least fld -: ty via Cs *)
+(* s |- C has least method -: ty via Cs *)
 val _ = add_rule {block_style = (AroundEachPhrase, (PP.CONSISTENT, 0)),
                   paren_style = OnlyIfNecessary,
                   fixity = Infix (NONASSOC, 460),
@@ -490,7 +492,7 @@ val get_class_constituents_def = Define`
 
 val sizeofmap_def = Define`
   sizeofmap s mdp =
-     FUN_FMAP (get_class_constituents s mdp) (FDOM s.classmap)
+     FUN_FMAP (get_class_constituents s mdp) (is_class_name s)
 `
 
 
@@ -520,6 +522,10 @@ val constituent_offsets_def = Define`
         MAP (\(n,c). (c, @off. offset (sizeofmap s) ccs n off)) nccs
 `;
 
+(* given a class name, and a mdp status, returns the list of direct components
+   along with their offsets, presented in the order in which they have to be
+   initialised - virtual bases (if any), direct bases, followed by
+   non-static data-members *)
 val init_order_offsets_def = Define`
   init_order_offsets s mdp cnm =
     let virts = if mdp then get_virtual_bases s cnm else [] in
@@ -534,49 +540,6 @@ val init_order_offsets_def = Define`
             alli
 `
 
-val (corder_trav_rules, corder_trav_ind, corder_trav_cases) = Hol_reln `
-   (!s a mdp cnm list.
-     cclist_trav s a (init_order_offsets s mdp cnm) list
-   ==>
-     corder_trav s mdp a cnm (list ++ [(a,cnm,[cnm])]))
-
-   /\
-
-   (!s a.
-     T
-   ==>
-     cclist_trav s a [] [])
-
-   /\
-
-   (!s a fldnm ty off.
-     ~class_type ty /\ cclist_trav s a rest list
-   ==>
-     cclist_trav s a ((NSD fldnm ty, off) :: rest) list)
-
-   /\
-
-   (!s a off cnm list1 list2 fldnm rest.
-     corder_trav s T (a + off) cnm list1 /\ cclist_trav s a rest list2
-   ==>
-     cclist_trav s a ((NSD fldnm (Class cnm), off) :: rest)
-                     (list1 ++ list2))
-
-   /\
-
-   (!s a off cnm list1 list2 rest.
-     corder_trav s F (a + off) cnm list1 /\ cclist_trav s a rest list2
-   ==>
-     cclist_trav s a ((DBase cnm, off) :: rest) (list1 ++ list2))
-
-   /\
-
-   (!s a off cnm list1 list2 rest.
-     corder_trav s F (a + off) cnm list1 /\ cclist_trav s a rest list2
-   ==>
-     cclist_trav s a ((VirtualBase cnm, off) :: rest) (list1 ++ list2))
-`;
-
 (* given derived class name C, state s, and path to (not necessarily
    immediate) base sub-class p, return the offset of the latter
    within an object of type C *)
@@ -588,47 +551,99 @@ val subobj_offset_def = Define`
                base_offset s C1 C3 + subobj_offset s (C3, (C3::t)))
 `
 
-(* BAD ASSUMPTION: no classes are abstract *)
-(* type-checking requires a variety of pieces of information, which we derive
-   from a state with this function *)
-val expr_type_comps_def = Define`
-  expr_type_comps s thisty =
-    <| class_fields :=
-          FUN_FMAP (\c. MAP (\ (n,ty). (SFName n, ty)) (THE (nsdmembers s c)))
-                   { c | ?v. c IN FDOM s.classmap /\
-                             (s.classmap ' c = SOME v) };
-       var_types := s.typemap ;
-       abs_classes := {} ;
-       this_type := thisty |>
+(* the fields belonging to this class specifically *)
+val get_fields_def = Define`
+  get_fields ci =
+          mapPartial
+            (\ (ce, b, p).
+               case ce of
+                  CFnDefn retty nm params body ->
+                     SOME (nm, Function retty (MAP SND params))
+               || FldDecl fld ty -> SOME (SFName fld, ty)
+               || _ -> NONE)
+            (FST ci).fields
 `;
 
-val MEM_splits = prove(
-  ``!l. MEM e l ==> ?pfx sfx. (l = pfx ++ (e :: sfx))``,
-  Induct THEN SRW_TAC [][] THENL [
-    MAP_EVERY Q.EXISTS_TAC [`[]`, `l`] THEN SRW_TAC [][],
-    RES_TAC THEN MAP_EVERY Q.EXISTS_TAC [`h::pfx`, `sfx`] THEN
-    SRW_TAC [][]
-  ]);
+val field_type_def = Define`
+  field_type ci sfld =
+    OPTION_MAP SND (FINDL (\ (nm, ty). nm = sfld) (get_fields ci))
+`;
 
-(* SANITY *)
-val hasfld_imp_lfi = store_thm(
-  "hasfld_imp_lfi",
-  ``s |- C has least fld -: ftype via p' /\ object_type ftype ==>
-    ?i. lookup_field_info
-          (MAP (\ (n,ty). (SFName n, ty))
-               (THE (nsdmembers s (LAST p'))))
-          fld
-          (i,ftype)``,
-  SRW_TAC [][fieldty_via_def, FieldDecls_def, nsdmembers_def] THEN
-  Cases_on `centry` THEN
-  FULL_SIMP_TAC (srw_ss()) [fieldtype_def, typesTheory.object_type_def,
-                            okfield_def] THEN
-  IMP_RES_TAC MEM_splits THEN
-  SRW_TAC [][fieldname_def] THEN
-  Q.HO_MATCH_ABBREV_TAC
-    `?i. lookup_field_info (L1 ++ (X,Y) :: L2) X (i,Y)` THEN
-  SRW_TAC [][staticsTheory.lookup_field_info_def] THEN
-  Q.EXISTS_TAC `LENGTH L1` THEN
-  SRW_TAC [ARITH_ss][rich_listTheory.EL_APPEND2])
+
+(* looks up an identifier corresponding to an object, and returns its type *)
+val elookup_type_def = Define`
+  (elookup_type env (IDFld id fld) =
+     case elookup_class env id of
+        NONE -> NONE
+     || SOME cenv -> (case (item cenv).info of
+                         NONE -> NONE
+                      || SOME ci -> field_type ci fld)) /\
+  (elookup_type env (IDConstant (b, [], n)) =
+     FLOOKUP ((item env).typemap) (SFName n)) /\
+  (elookup_type env (IDConstant (b, h :: t, n)) =
+     case FLOOKUP (map env) h of
+        NONE -> NONE
+     || SOME e' -> elookup_type e' (IDConstant (b, t, n))) /\
+  (elookup_type env (IDTempCall (TemplateConstant (b, [], n)) targs) =
+     FLOOKUP ((item env).typemap) (SFTempCall n targs)) /\
+  (elookup_type env (IDTempCall (TemplateConstant (b, h :: t, n)) targs) =
+     case FLOOKUP (map env) h of
+        NONE -> NONE
+     || SOME e' -> elookup_type e' (IDTempCall
+                                    (TemplateConstant(b, t, n))
+                                    targs))
+`;
+
+(* looks up an object identifier and returns its address *)
+val elookup_addr_def = Define`
+  (* must be a SFName, a template id could only be to a function, which is
+     not an object *)
+  (elookup_addr env (IDFld id (SFName fld)) =
+     case elookup_class env id of
+        NONE -> NONE
+     || SOME cenv -> FLOOKUP (item cenv).statvars fld) /\
+  (elookup_addr env (IDConstant (b, [], n)) = FLOOKUP (item env).varmap n) /\
+  (elookup_addr env (IDConstant (b, h::t, n)) =
+     case FLOOKUP (map env) h of
+        NONE -> NONE
+     || SOME e' -> elookup_addr e' (IDConstant(b, t, n))) /\
+  (elookup_addr env _ = NONE)
+`;
+
+(* state-based, as opposed to environment-based, lookup functions *)
+val lift_lookup_def = Define`
+  lift_lookup f s id = if is_abs_id id then f s.genv id
+                       else f s.env id
+`;
+
+val lookup_addr_def = Define` lookup_addr =  lift_lookup elookup_addr `;
+val lookup_type_def = Define` lookup_type =  lift_lookup elookup_type `;
+val lookup_class_def = Define`lookup_class = lift_lookup elookup_class `;
+
+(* looks up a fully-qualified non-static data member field (e.g., C::fld) and
+   finds its offset within that class.
+
+*)
+val lookup_offset_def = Define`
+  (lookup_offset s mdp (IDFld id (SFName fld)) =
+     let coffs = constituent_offsets s mdp id
+     in
+       case FINDL (\ (cc, off). ?ty. cc = NSD fld ty) coffs of
+          NONE -> NONE
+       || SOME (cc, off) -> SOME off) /\
+  (lookup_offset s mdp _ = NONE)
+`;
+
+
+(* looks up a fully-qualified field (e.g., C::fld) and finds its type *)
+val lookup_field_type_def = Define`
+  (lookup_field_type s (IDFld id sfld) =
+    case lookup_class s id of
+       NONE -> NONE
+    || SOME cenv -> (case (item cenv).info of
+                        NONE -> NONE
+                     || SOME ce -> field_type ce sfld)) /\
+  (lookup_field_type s _ = NONE)
+`;
 
 val _ = export_theory();
