holsrcs/staticsScript.sml
@@ -13,98 +13,11 @@ open arithmeticTheory pred_setTheory integerTheory
 local open wordsTheory integer_wordTheory finite_mapTheory in end
 
 (* C++ ancestor theories  *)
-open typesTheory memoryTheory expressionsTheory
+open typesTheory memoryTheory expressionsTheory operatorsTheory
+     class_infoTheory
 
 val _ = new_theory "statics";
 
-(* conditions on whether or not a conditional expressions has a given type *)
-(* In C++ Standard, this is 5.16 *)
-val cond_typing_conds_def = Define`
-  cond_typing_conds (gty, t1, t2, restype) =
-      scalar_type gty /\
-      (arithmetic_type t1 /\ arithmetic_type t2 /\
-       (restype = ua_conversions t1 t2) \/
-      (?s. (t1 = Class s) /\ (t1 = t2) /\ (t1 = restype)) \/
-      pointer_type t1 /\ pointer_type t2 /\
-      ((t1 = t2) /\ (restype = t1) \/
-       Ptr Void IN {t1; t2} /\ (restype = Ptr Void)) \/
-      (t1 = Void) /\ (t2 = t1) /\ (restype = t1))
-`;
-
-(* SANITY *)
-val cond_typing_conds_det = store_thm(
-  "cond_typing_conds_det",
-  ``!gty t1 t2 rt1 rt2.
-       cond_typing_conds (gty, t1, t2, rt1) ==>
-       cond_typing_conds (gty, t1, t2, rt2) ==>
-       (rt1 = rt2)``,
-  SRW_TAC [][cond_typing_conds_def] THEN
-  TRY (FULL_SIMP_TAC (srw_ss()) [arithmetic_type_def] THEN NO_TAC) THEN
-  METIS_TAC [type_classes])
-
-(* SANITY *)
-val cond_typing_wellformed = store_thm(
-  "cond_typing_wellformed",
-  ``!gty acs t1 t2 rt.
-       cond_typing_conds (gty, t1, t2, rt) /\
-       wf_type acs t1 /\ wf_type acs t2 ==>
-       wf_type acs rt``,
-  SRW_TAC [][cond_typing_conds_def] THEN
-  SRW_TAC [][typesTheory.ua_converted_types_well_formed])
-
-val arithmetic_pair_type_def = Define`
-  arithmetic_pair_type t1 t2 t =
-      arithmetic_type t1 /\ arithmetic_type t2 /\
-      (t = ua_conversions t1 t2)
-`;
-
-val binary_op_type_def = Define`
-    (binary_op_type CPlus t1 t2 t =
-      arithmetic_pair_type t1 t2 t \/
-      (pointer_type t1 /\ integral_type t2 /\ (t = t1)) \/
-      (integral_type t1 /\ pointer_type t2 /\ (t = t2))) /\
-    (binary_op_type CMinus t1 t2 t =
-      arithmetic_pair_type t1 t2 t \/
-      (pointer_type t1 /\ integral_type t2 /\ (t = t1)) \/
-      (pointer_type t1 /\ (t1 = t2) /\ (t = ptrdiff_t))) /\
-    (binary_op_type CLess t1 t2 t =
-      arithmetic_type t1 /\ arithmetic_type t2 /\ (t = Signed Int) \/
-      pointer_type t1 /\ (t1 = t2) /\ (t = Signed Int)) /\
-    (binary_op_type CGreat t1 t2 t =
-      arithmetic_type t1 /\ arithmetic_type t2 /\ (t = Signed Int) \/
-      pointer_type t1 /\ (t1 = t2) /\ (t = Signed Int)) /\
-    (binary_op_type CLessE t1 t2 t =
-      arithmetic_type t1 /\ arithmetic_type t2 /\ (t = Signed Int) \/
-      pointer_type t1 /\ (t1 = t2) /\ (t = Signed Int)) /\
-    (binary_op_type CGreatE t1 t2 t =
-      arithmetic_type t1 /\ arithmetic_type t2 /\ (t = Signed Int) \/
-      pointer_type t1 /\ (t1 = t2) /\ (t = Signed Int)) /\
-    (binary_op_type CEq t1 t2 t =
-      arithmetic_type t1 /\ arithmetic_type t2 /\ (t = Signed Int) \/
-      pointer_type t1 /\ (t1 = t2) /\ (t = Signed Int) \/
-      pointer_type t1 /\ pointer_type t2 /\
-      {Ptr Void} SUBSET {t1; t2} /\ (t = Signed Int)) /\
-    (binary_op_type CNotEq t1 t2 t =
-      arithmetic_type t1 /\ arithmetic_type t2 /\ (t = Signed Int) \/
-      pointer_type t1 /\ (t1 = t2) /\ (t = Signed Int) \/
-      pointer_type t1 /\ pointer_type t2 /\
-      {Ptr Void} SUBSET {t1; t2} /\ (t = Signed Int)) /\
-    (binary_op_type CTimes t1 t2 t = arithmetic_pair_type t1 t2 t) /\
-    (binary_op_type CDiv t1 t2 t = arithmetic_pair_type t1 t2 t) /\
-    (binary_op_type CMod t1 t2 t =
-      integral_type t1 /\ integral_type t2 /\
-      (t = ua_conversions t1 t2))
-`
-
-val unary_op_type_def = Define`
-    (unary_op_type CUnPlus t0 t =
-      arithmetic_type t0 /\ (t = integral_promotions t0)) /\
-    (unary_op_type CUnMinus t0 t =
-      arithmetic_type t0 /\ (t = integral_promotions t0)) /\
-    (unary_op_type CComp t0 t =
-      integral_type t0 /\ (t = integral_promotions t0)) /\
-    (unary_op_type CNot t0 t = scalar_type t0 /\ (t = Signed Int))
-`
 
 (* t1 is the type of the lvalue, t2 is the type of the RHS.
    ass_type_conds checks whether the two are compatible. *)
@@ -125,18 +38,6 @@ val (ass_type_conds,_) = Defn.tprove(
 val _ = save_thm("ass_type_conds", ass_type_conds);
 
 
-(* SANITY *)
-val ops_dont_produce_arrays = store_thm(
-  "ops_dont_produce_arrays",
-  ``(!f t1 t2 rt. binary_op_type f t1 t2 rt ==> ~array_type rt) /\
-    (!f t0 rt.    unary_op_type f t0 rt ==> ~array_type rt)``,
-  CONJ_TAC THEN GEN_TAC THENL [
-    STRUCT_CASES_TAC (Q.SPEC `f` expressionsTheory.c_binops_nchotomy),
-    STRUCT_CASES_TAC (Q.SPEC `f` expressionsTheory.c_unops_nchotomy)
-  ] THEN SRW_TAC [][binary_op_type_def, unary_op_type_def,
-    arithmetic_pair_type_def] THEN
-  METIS_TAC [type_classes, integral_type_def, integral_promotions_safe,
-             ua_conversions_safe]);
 
 val lookup_field_info_def = Define`
   lookup_field_info s n (idx,t) = idx < LENGTH s /\ (EL idx s = (n,t))
@@ -181,16 +82,20 @@ val nodups_lfi_det = store_thm(
              DECIDE ``0n < i /\ 0 < i' /\ (i - 1 = i' - 1) ==> (i = i')``]);
 
 
-val _ = Hol_datatype `expr_value_type = LValue | RValue`;
+(* BAD ASSUMPTION: no classes are abstract *)
+val abs_classes_def = Define`
+  abs_classes (s:state) = ({} : CPP_ID set)
+`;
+val _ = temp_add_record_field ("abs_classes", ``abs_classes``)
 
-val _ = Hol_datatype `
-  static_info = <|
-    class_fields : class_spec |-> (StaticField # CPP_Type) list ;
-    var_types    : CPPname |-> CPP_Type ;
-    abs_classes  : class_spec set ;
-    this_type    : CPP_Type option
-  |>
-`
+val this_type_def = Define`
+  this_type s = case s.thisvalue of
+                  SOME (ECompVal bytes (Ptr ty)) -> SOME ty
+                || _ -> NONE
+`;
+val _ = temp_add_record_field ("this_type", ``this_type``)
+
+val _ = Hol_datatype `expr_value_type = LValue | RValue`;
 
 val (expr_type_rules, expr_type_ind, expr_type_cases) = Hol_reln`
 
@@ -215,20 +120,21 @@ val (expr_type_rules, expr_type_ind, expr_type_cases) = Hol_reln`
       wf_type si.abs_classes t ==>
       expr_type si RValue (Cnullptr t) (Ptr t)) /\
 
-  (!si vmap n.
-      (vmap = si.var_types) /\
-      wf_type si.abs_classes (vmap ' n) /\ ~(vmap ' n = Void) /\ n IN FDOM vmap
-         ==>
-      expr_type si LValue (Var n) (vmap ' n)) /\
+  (!s n ty.
+      (lookup_type s n = SOME ty) /\
+      wf_type (abs_classes s) ty /\
+      ~(ty = Void)
+    ==>
+      expr_type s LValue (Var n) ty) /\
 
   (!si n t t' p.
-      wf_type si.abs_classes t /\ ~(t = Void) /\
+      wf_type (abs_classes si) t /\ ~(t = Void) /\
       (t' = if p = [] then t else Class (LAST p))
          ==>
       expr_type si LValue (LVal n t p) t') /\
 
   (!si v t.
-      wf_type si.abs_classes t /\ ~array_type t
+      wf_type (abs_classes si) t /\ ~array_type t
          ==>
       expr_type si RValue (ECompVal v t) t) /\
 
@@ -237,7 +143,7 @@ val (expr_type_rules, expr_type_ind, expr_type_cases) = Hol_reln`
             expr_type s RValue (RValreq e) t) /\
 
   (!si e t t0.
-      wf_type si.abs_classes t /\ (scalar_type t \/ (t = Void)) /\
+      wf_type (abs_classes si) t /\ (scalar_type t \/ (t = Void)) /\
       expr_type si RValue e t0
           ==>
       expr_type si RValue (Cast t e) t) /\
@@ -248,7 +154,7 @@ val (expr_type_rules, expr_type_ind, expr_type_cases) = Hol_reln`
      compatible with argument-types of function *)
   (!s e1 e2 rt args.
        expr_type s RValue e1  (Function rt args) /\
-       expr_typel s e2 args
+       listRel (expr_type s RValue) e2 args
           ==>
        expr_type s RValue (FnApp e1 e2) rt) /\
 
@@ -304,28 +210,27 @@ val (expr_type_rules, expr_type_ind, expr_type_cases) = Hol_reln`
   (!s e t. expr_type s LValue e t ==>
            expr_type s RValue (Addr e) (Ptr t)) /\
 
-  (!si e sn n i t.
-       expr_type si LValue e (Class sn) /\ sn IN FDOM si.class_fields /\
-       lookup_field_info (si.class_fields ' sn) n (i,t) ==>
-       expr_type si LValue (SVar e n) t) /\
+  (!s e c1 c2 sfld ty.
+       expr_type s LValue e (Class c1) /\
+       s |- c2 <= c1 /\
+       (lookup_field_type s (IDFld c2 sfld) = SOME ty)
+     ==>
+       expr_type s LValue (SVar e (IDFld c2 sfld)) ty) /\
 
-  (!si e sn n i t.
-       expr_type si RValue e (Class sn) /\ sn IN FDOM si.class_fields /\
-       lookup_field_info (si.class_fields ' sn) n (i, t) /\ ~array_type t ==>
-       expr_type si RValue (SVar e n) t) /\
+  (!s e c1 c2 sfld ty.
+       expr_type s RValue e (Class c1) /\
+       s |- c2 <= c1 /\
+       (lookup_field_type s (IDFld c2 sfld) = SOME ty) /\
+       ~array_type ty
+     ==>
+       expr_type s RValue (SVar e (IDFld c2 sfld)) ty)
+
+  /\
 
   (!s e1 e2 t0 t.
        expr_type s RValue e2 t /\
        expr_type s RValue e1 t0 ==>
-       expr_type s RValue (CommaSep e1 e2) t) /\
-
-  (!s. expr_typel s [] []) /\
-
-  (!s hde hdt tle tlt.
-       expr_type s RValue hde  hdt /\
-       expr_typel s tle tlt
-         ==>
-       expr_typel s (hde :: tle) (hdt :: tlt))
+       expr_type s RValue (CommaSep e1 e2) t)
 `
 
 infix >-
@@ -346,17 +251,9 @@ val rvalue_typing = save_thm(
   LIST_CONJ (map (GEN_ALL o (fn t =>
     (ONCE_REWRITE_CONV [expr_type_cases] THENC SIMP_CONV (srw_ss()) [])
     ``expr_type env RValue ^t t``)) e_cases));
-val list_etype_rewrites =
-  CONJ (GEN_ALL
-          ((ONCE_REWRITE_CONV [expr_type_cases] THENC
-            SIMP_CONV (srw_ss()) []) ``expr_typel s [] t``))
-       (GEN_ALL
-          ((ONCE_REWRITE_CONV [expr_type_cases] THENC
-            SIMP_CONV (srw_ss()) [])
-           ``expr_typel s (e:: es) t``))
 val expr_type_rewrites = save_thm(
   "expr_type_rewrites",
-  LIST_CONJ [lvalue_typing, rvalue_typing, list_etype_rewrites]);
+  LIST_CONJ [lvalue_typing, rvalue_typing]);
 val expr_typing = save_thm(
   "expr_typing",
   LIST_CONJ (
@@ -364,24 +261,6 @@ val expr_typing = save_thm(
       (fn t => GEN_ALL (
         (ONCE_REWRITE_CONV [expr_type_cases] THENC SIMP_CONV (srw_ss()) [])
       ``expr_type senv v ^t t``)) e_cases));
-
-(* SANITY *)
-val unary_op_type_det = store_thm(
-  "unary_op_type_det",
-  ``!f t0 t1.
-       unary_op_type f t0 t1 ==>
-       (!t2. unary_op_type f t0 t2 ==> (t1 = t2))``,
-  GEN_TAC THEN Cases_on `f` THEN SIMP_TAC (srw_ss()) [unary_op_type_def]);
-
-(* SANITY *)
-val binary_op_type_det = store_thm(
-  "binary_op_type_det",
-  ``!f t1 t2 t.
-       binary_op_type f t1 t2 t ==>
-       (!t'. binary_op_type f t1 t2 t' ==> (t' = t))``,
-  Cases THEN
-  SIMP_TAC (srw_ss()) [binary_op_type_def, arithmetic_pair_type_def] THEN
-  SRW_TAC [][] THEN METIS_TAC [type_classes]);
 
 val lvalue_rvalue_nonarray = store_thm(
   "lvalue_rvalue_nonarray",
@@ -392,88 +271,69 @@ val lvalue_rvalue_array = store_thm(
   ``expr_type s LValue e (Array bt n) ==> expr_type s RValue e (Ptr bt)``,
   PROVE_TAC [expr_type_rules]);
 
-
-val wf_strmap_def = Define`
-  wf_strmap smap = !s. s IN FDOM smap ==> nodup_flds (smap ' s)
-`;
-
 (* SANITY : only one type possible *)
 val expr_type_det_lemma = prove(
   ``(!s v e t.
        expr_type s v e t ==>
           has_no_undefineds e ==>
-          wf_strmap s.class_fields ==>
           (!t'. expr_type s v e t' = (t' = t)) /\
           ((v = LValue) ==>
            (!bt n. (t = Array bt n) ==>
                    !t'. expr_type s RValue e t' = (t' = Ptr bt)) /\
-           (~array_type t ==> !t'. expr_type s RValue e t' = (t' = t)))) /\
-    (!s e t. expr_typel s e t ==>
-               wf_strmap s.class_fields ==>
-               ALL_EL has_no_undefineds e ==>
-               (!t'. expr_typel s e t' = (t' = t)))``,
+           (~array_type t ==> !t'. expr_type s RValue e t' = (t' = t))))``,
   HO_MATCH_MP_TAC expr_type_ind THEN
   SRW_TAC [ETA_ss][lvalue_typing] THEN
   ASM_SIMP_TAC (srw_ss()) [expr_type_rewrites] THEN
   FULL_SIMP_TAC (srw_ss()) [wf_type_def] THEN
   TRY (METIS_TAC [array_type_def, wf_type_def, unary_op_type_det,
-                  binary_op_type_det, cond_typing_conds_det, wf_strmap_def,
+                  binary_op_type_det, cond_typing_conds_det,
                   nodups_lfi_det, TypeBase.one_one_of ``:CPP_Type``,
-                  lvalue_rvalue_nonarray]))
+                  lvalue_rvalue_nonarray]) THEN
+  SRW_TAC [][EQ_IMP_THM] THEN
+  REPEAT (POP_ASSUM (fn th => if free_in ``e2:CExpr list`` (concl th) then
+                                MP_TAC th
+                              else ALL_TAC)) THEN
+  Q.ID_SPEC_TAC `args` THEN Induct_on `e2` THEN
+  SRW_TAC [][listTheory.listRel_CONS]);
 val expr_type_det0 = save_thm(
   "expr_type_det0",
   SIMP_RULE (srw_ss() ++ DNF_ss) [] expr_type_det_lemma);
 val expr_type_det = store_thm(
   "expr_type_det",
   ``!e v s t1 t2.
-      expr_type s v e t1 /\ expr_type s v e t2 /\ wf_strmap s.class_fields /\
-      has_no_undefineds e ==>
+      expr_type s v e t1 /\ expr_type s v e t2 /\ has_no_undefineds e ==>
       (t1 = t2)``,
   METIS_TAC [expr_type_det0])
 
-val expr_type_lists0 = prove(
-  ``(!s tlr. expr_typel s [] tlr = (tlr = [])) /\
-    (!s elr. expr_typel s elr [] = (elr = [])) /\
-    (!s e el tlr.
-               expr_typel s (e::el) tlr =
-               ?t tl. (tlr = t::tl) /\
-                      expr_type s RValue e t /\
-                      expr_typel s el tl) /\
-    (!s elr t tl.
-               expr_typel s elr (t::tl) =
-               ?e el. (elr = e::el) /\
-                      expr_type s RValue e t /\
-                      expr_typel s el tl)``,
-  REPEAT STRIP_TAC THEN
-  CONV_TAC (LHS_CONV (ONCE_REWRITE_CONV [expr_type_cases])) THEN
-  SIMP_TAC (srw_ss()) [])
-
-val expr_type_lists_append = prove(
-  ``(!s el1 el2 tlr.
-               expr_typel s (APPEND el1 el2) tlr =
-               ?tl1 tl2. (tlr = APPEND tl1 tl2) /\
-                         expr_typel s el1 tl1 /\
-                         expr_typel s el2 tl2) /\
-    (!s tl1 tl2 elr.
-               expr_typel s elr (APPEND tl1 tl2) =
-               ?el1 el2. (elr = APPEND el1 el2) /\
-                         expr_typel s el1 tl1 /\
-                         expr_typel s el2 tl2)``,
-  CONJ_TAC THENL [
-    Induct_on `el1` THEN SRW_TAC [][expr_type_lists0] THEN
-    ASM_SIMP_TAC (srw_ss() ++ DNF_ss) [] THEN METIS_TAC [],
-    Induct_on `tl1` THEN SRW_TAC [][expr_type_lists0] THEN
-    ASM_SIMP_TAC (srw_ss() ++ DNF_ss) [] THEN METIS_TAC []
+val MEM_splits = prove(
+  ``!l. MEM e l ==> ?pfx sfx. (l = pfx ++ (e :: sfx))``,
+  Induct THEN SRW_TAC [][] THENL [
+    MAP_EVERY Q.EXISTS_TAC [`[]`, `l`] THEN SRW_TAC [][],
+    RES_TAC THEN MAP_EVERY Q.EXISTS_TAC [`h::pfx`, `sfx`] THEN
+    SRW_TAC [][]
   ]);
 
-val expr_type_lists = save_thm(
-  "expr_type_lists",
-  CONJ expr_type_lists0 expr_type_lists_append);
-val expr_typel_list_lengths = store_thm(
-  "expr_typel_list_lengths",
-  ``!s el tl. expr_typel s el tl ==> (LENGTH el = LENGTH tl)``,
-  Induct_on `el` THEN SRW_TAC [][expr_type_lists] THEN
-  SRW_TAC [][] THEN METIS_TAC [])
+(* SANITY *)
+val hasfld_imp_lfi = store_thm(
+  "hasfld_imp_lfi",
+  ``s |- C has least fld -: ftype via p' /\ object_type ftype ==>
+    ?i. lookup_field_info
+          (MAP (\ (n,ty). (SFName n, ty))
+               (THE (nsdmembers s (LAST p'))))
+          fld
+          (i,ftype)``,
+  SRW_TAC [][fieldty_via_def, FieldDecls_def, nsdmembers_def] THEN
+  Cases_on `centry` THEN
+  FULL_SIMP_TAC (srw_ss()) [fieldtype_def, typesTheory.object_type_def,
+                            okfield_def] THEN
+  IMP_RES_TAC MEM_splits THEN
+  SRW_TAC [][fieldname_def] THEN
+  Q.HO_MATCH_ABBREV_TAC
+    `?i. lookup_field_info (L1 ++ (X,Y) :: L2) X (i,Y)` THEN
+  SRW_TAC [][lookup_field_info_def] THEN
+  Q.EXISTS_TAC `LENGTH L1` THEN
+  SRW_TAC [ARITH_ss][rich_listTheory.EL_APPEND2])
+
 
 val _ = export_theory();
 
