holsrcs/environmentsScript.sml
@@ -1,0 +1,222 @@
+(* C++ environments, handling namespaces and nested classes *)
+
+(* Michael Norrish *)
+
+(* pro-forma *)
+open HolKernel boolLib Parse bossLib BasicProvers
+open boolSimps
+
+(* Standard HOL ancestory theories *)
+open arithmeticTheory pred_setTheory integerTheory
+local
+  open wordsTheory integer_wordTheory finite_mapTheory fmaptreeTheory
+in end
+
+(* C++ ancestor theories  *)
+open utilsTheory typesTheory memoryTheory expressionsTheory statementsTheory
+
+val _ = new_theory "environments";
+
+
+(* In the classmap and gclassmap fields, use the NONE value to
+   indicate a class has an incomplete declaration.  Can't use the
+   empty list of fields for C++, as C++ allows declaration of empty
+   structs/classes (unlike C) (9 p1).
+
+   NOTE, moreover that an empty C++ struct has non-zero size. (9 p3) *)
+
+
+(* those sorts of things that can get implicitly declared and defined by
+   the implementation if the user does not provide them *)
+val _ = Hol_datatype`
+  implicitly_definable = DefaultConstructor
+                       | Destructor
+                       | CopyConstructor
+                       | CopyAssignment
+`;
+
+(* when a class name is looked up, it may get
+     - that the name is not in the domain of the map, which means that the
+       name is not the name of a class at all
+     - the name maps to NONE, which means it has been declared only,
+       as in
+          class foo;
+     - the name maps to SOME(cinfo, user_provided) where cinfo is the
+       information about the class, and user_provided is the set of things
+       that were given by the user (and didn't need filling in by the
+       implementation)
+*)
+
+val _ = type_abbrev("state_class_info",
+                    ``:(class_info # implicitly_definable set) option``)
+
+
+val _ = type_abbrev("construction_locn",
+                    ``:addr # class_spec # class_spec list``)
+
+val _ = Hol_datatype`
+  class_envinfo = <|
+    (* ironically, the location of the static variables is only available
+       dynamically, as classes are initialised *)
+    statvars : string |-> addr # CPP_ID list ;
+    info     : state_class_info ;
+    refs     : string # addr |-> addr # CPP_ID list
+|>`
+
+
+val _ = type_abbrev ("class_env", ``:(StaticField,class_envinfo)fmaptree``)
+
+val _ = Hol_datatype`
+  envinfo = <| varmap   : string |-> addr # CPP_ID list ;
+               typemap  : StaticField |-> CPP_Type ;
+               classenv : StaticField |-> class_env ;
+               funs     : StaticField |-> CPP_ID (* function's fullname *)
+|>`;
+
+(* strings are the keys here, because these are ever-deepening
+   namespace identifiers *)
+val _ = type_abbrev ("environment", ``:(string,envinfo)fmaptree``)
+
+val empty_env_def = Define`
+  empty_env = FTNode <| varmap := FEMPTY ;
+                        typemap := FEMPTY ;
+                        classenv := FEMPTY ;
+                        funs := FEMPTY |>
+                     FEMPTY
+`;
+
+val lookup_nspace_def = Define`
+  (lookup_nspace env [] = env) /\
+  (lookup_nspace env (h::t) = lookup_nspace (map env ' h) t)
+`;
+
+val elookup_class_def = Define`
+  (elookup_class env (IDFld id fld) =
+     case elookup_class env id of
+        NONE -> NONE
+     || SOME cenv -> FLOOKUP (map cenv) fld) /\
+  (elookup_class env (IDConstant (b, [], n)) =
+      FLOOKUP ((item env).classenv) (SFName n)) /\
+  (elookup_class env (IDConstant (b, h :: t, n)) =
+      case FLOOKUP (map env) h of
+         NONE -> NONE
+      || SOME m -> elookup_class m (IDConstant(b, t, n))) /\
+  (elookup_class env (IDTempCall (TemplateConstant (b, [], n)) targs) =
+      FLOOKUP ((item env).classenv) (SFTempCall n targs)) /\
+  (elookup_class env (IDTempCall (TemplateConstant (b, h::t, n)) targs) =
+      case FLOOKUP (map env) h of
+         NONE -> NONE
+      || SOME m -> elookup_class m
+                         (IDTempCall (TemplateConstant (b, t, n)) targs)) /\
+  (elookup_class env _ = NONE)
+`;
+
+val is_class_name_env_def = Define`
+  (is_class_name_env env id = ?c. elookup_class env id = SOME c)
+`;
+
+
+val update_classenv_def = Define`
+  (update_classenv [] i (cenv : StaticField |-> class_env) = NONE) /\
+  (update_classenv [h] i cenv =
+     SOME (cenv |+ (h, FTNode <| info := SOME i ;
+                                 statvars := FEMPTY ;
+                                 refs := FEMPTY |>
+                              FEMPTY))) /\
+  (update_classenv (h::t) i cenv =
+     if h IN FDOM cenv then
+       case update_classenv t i (map (cenv ' h)) of
+          NONE -> NONE
+       || SOME ce' -> SOME (cenv |+ (h, FTNode (item (cenv ' h)) ce'))
+     else NONE)
+`;
+
+val update_class_def = Define`
+  update_class id i env =
+     let (bid, sfs) = strip_field id
+     in
+       case strip_nspaces bid of
+          NONE -> NONE
+       || SOME ((b, ns), sf) ->
+            fupd_at_path ns
+              (\ft. case update_classenv (sf::sfs) i (item ft).classenv of
+                       NONE -> NONE
+                    || SOME ce' -> SOME (FTNode (item ft with classenv := ce')
+                                                (map ft)))
+              env
+`
+
+
+val id_GSPEC_cases = store_thm(
+  "id_GSPEC_cases",
+  ``{ id | P id } =
+      { IDVar s | P (IDVar s) } UNION
+      { IDFld id sf | P (IDFld id sf) } UNION
+      { IDTempCall tid targs | P (IDTempCall tid targs) } UNION
+      { IDConstant tn | P (IDConstant tn) }``,
+  SRW_TAC [][EXTENSION] THEN Cases_on `x` THEN SRW_TAC [][]);
+
+val option_case_lemma = prove(
+  ``(option_case NONE f x = SOME y) = ?z. (x = SOME z) /\ (f z = SOME y)``,
+  Cases_on `x` THEN SRW_TAC [][]);
+
+(* SANITY *)
+(* empty list is an error case *)
+val class_part_def = Define`
+  (class_part (IDFld id fld) =
+     case class_part id of
+        [] -> []
+     || list -> list ++ [fld]) /\
+  (class_part (IDConstant(b,l,n)) = [SFName n]) /\
+  (class_part (IDTempCall (TemplateConstant(b,l,n)) targs) =
+              [SFTempCall n targs]) /\
+  (class_part _ = [])
+`;
+
+val option_case_lemma2 = prove(
+  ``option_case NONE (\x. SOME x) y = y``,
+  Cases_on `y` THEN SRW_TAC [][]);
+
+val list_case_lemma = prove(
+  ``(list_case NONE f x = SOME y) =
+    ?h t. (x = h :: t) /\ (f h t = SOME y)``,
+  Cases_on `x` THEN SRW_TAC [][]);
+
+val elookup_class_apply_path = store_thm(
+  "elookup_class_apply_path",
+  ``!env id.
+       elookup_class env id =
+          case class_part id of
+             [] -> NONE
+          || h::t -> (case apply_path (SND (id_namespaces id)) env of
+                         NONE -> NONE
+                      || SOME e -> (case FLOOKUP (item e).classenv h of
+                                       NONE -> NONE
+                                    || SOME ce -> apply_path t ce))``,
+  HO_MATCH_MP_TAC (theorem "elookup_class_ind") THEN
+  SRW_TAC [][elookup_class_def, fmaptreeTheory.apply_path_def, class_part_def,
+             typesTheory.id_namespaces_def, typesTheory.tid_namespaces_def,
+             option_case_lemma2] THEN
+  TRY (SRW_TAC [][finite_mapTheory.FLOOKUP_DEF] THEN NO_TAC) THEN
+  Cases_on `class_part id` THEN SRW_TAC [][] THEN
+  Cases_on `apply_path (SND (id_namespaces id)) env` THEN SRW_TAC [][] THEN
+  Cases_on `FLOOKUP (item x).classenv h` THEN SRW_TAC [][] THEN
+  SRW_TAC [][fmaptreeTheory.apply_path_SNOC]);
+
+(* tricksy
+val env_classes_FINITE = store_thm(
+  "env_classes_FINITE",
+  ``!env. FINITE { id | is_class_name_env env id }``,
+  SIMP_TAC (srw_ss()) [is_class_name_env_def] THEN
+  SRW_TAC [DNF_ss][elookup_class_apply_path, option_case_lemma,
+                   list_case_lemma] THENL [
+    Q_TAC SUFF_TAC `{IDVar s | F} = {}` THEN1 SRW_TAC [][] THEN
+    SRW_TAC [][EXTENSION],
+    SRW_TAC [][option_case_lemma]
+*)
+
+
+
+
+val _ = export_theory()
+
