holsrcs/name_resolutionScript.sml
@@ -1,0 +1,148 @@
+(* Resolution of names within a sequence of external declarations *)
+
+(* (Can be viewed as a phase of compilation) *)
+
+(* Michael Norrish *)
+
+(* pro-forma *)
+open HolKernel boolLib Parse bossLib BasicProvers
+open boolSimps
+
+
+(* Standard HOL ancestory theories *)
+open arithmeticTheory pred_setTheory integerTheory
+local open wordsTheory integer_wordTheory finite_mapTheory in end
+
+(* C++ ancestor theories  *)
+open typesTheory memoryTheory expressionsTheory staticsTheory class_infoTheory
+open aggregatesTheory declaration_dynamicsTheory
+local
+  open side_effectsTheory statesTheory operatorsTheory overloadingTheory
+in end
+
+val _ = new_theory "name_resolution";
+
+val _ = set_trace "inddef strict" 1
+
+
+(* non-function field resolution rule
+(* Note how the path p is used:
+     - to figure out the static type of the l-value (LAST p)
+     - to derive the path from the most-derived class to the sub-object
+       enclosing the field.  The offset is calculated with respect to
+       this because the sub-object could be anywhere, and might be virtual.
+
+
+       subobject of the original LVal is ignored.  This is because
+   only functions can get a "virtual" treatment.
+   This doesn't mean that a field reference can't be to an ancestor's field.
+
+*)
+(!s cnm fld ftype Cflds se offn i a p p'.
+     s |- LAST p has least fld -: ftype via p' /\
+     (Cflds = THE (nsdmembers s (LAST p'))) /\
+     object_type ftype /\
+     lookup_field_info (MAP (\ (n,ty). (SFName n, ty)) Cflds) fld (i,ftype) /\
+     offset (sizeofmap s) (MAP (UNCURRY NSD) Cflds) i offn
+   ==>
+     ^mng (mExpr (SVar (LVal a (Class cnm) p) fld) se) s
+          (s, ev (LVal (a + subobj_offset s (cnm, p ^ p') + offn) ftype
+                       (default_path ftype)) se))
+*)
+
+
+(* ----------------------------------------------------------------------
+    how to evaluate a sequence of external declarations
+   ---------------------------------------------------------------------- *)
+
+(* split a name into a class::fld part *)
+val class_fld_split_def = Define`
+  class_fld_split (IDFld id fld) = (id, fld)
+`;
+
+
+(* if the evaluation can't get the list of external declarations to the
+   empty list, this is (implicitly) an occurrence of undefined behaviour *)
+val (emeaning_rules, emeaning_ind, emeaning_cases) = Hol_reln`
+
+(* RULE-ID: global-fndefn *)
+(!s0 s fval name rettype params body ftype edecls.
+     installfn s0 Ptr rettype name params body fval s /\
+     ~(name IN FDOM s.typemap) /\ ~is_class_name s0 name /\
+     (ftype = Function rettype (MAP SND params))
+   ==>
+     emeaning
+       (FnDefn rettype name params body :: edecls) s
+       (s with <| typemap updated_by (\tm. tm |+ (name, ftype)) |>,
+        edecls))
+
+   /\
+
+(* RULE-ID: member-fndefn *)
+(* The first MEM clause looks up the assumed declaration, and gets
+   static-ness and protection information there.
+   The second MEM clauses checks that this is not a duplicate definition
+     (this is a static check, one that would be performed by the compiler
+      if the duplication occurred within a single translation unit, or by
+      the linker if it occurred across multiple units)
+*)
+(!rettype userdefs name params body edecls s0 s cinfo staticp prot cpart base.
+     is_class_name s0 name /\
+     ((cpart, base) = class_fld_split name) /\
+     (SOME (cinfo, userdefs) = s0.classmap ' cpart) /\
+     (?pms'.
+         MEM (CFnDefn rettype base pms' NONE, staticp, prot)
+             cinfo.fields /\
+         (MAP SND pms' = MAP SND params)) /\
+     (!bdy' rettype' statp prot pms'.
+         MEM (CFnDefn rettype' base pms' bdy', statp, prot) cinfo.fields
+           ==>
+         ~(MAP SND pms' = MAP SND params)) /\
+     install_member_functions cpart s0
+                              [(CFnDefn rettype base params (SOME body),
+                                staticp, prot)]
+                              s
+   ==>
+     emeaning (FnDefn rettype name params body :: edecls) s0
+              (s, edecls))
+
+   /\
+
+(* RULE-ID: global-declmng *)
+(!s0 s d0 ds edecls.
+     declmng meaning copy2globals (d0, s0) (ds, s)
+   ==>
+     emeaning (Decl d0 :: edecls) s0 (s, MAP Decl ds ++ edecls))
+
+   /\
+
+(* RULE-ID: global-class-declaration *)
+(*   one might argue that this is a useless rule to have dynamically, as
+     class declarations are only made for the benefit of static type-checking
+*)
+(!name edecls s0.
+     T
+   ==>
+     emeaning
+        (Decl (VStrDec name NONE) :: edecls) s0
+        (copy2globals
+           (s0 with classmap updated_by (\sm. sm |+ (name, NONE))),
+         edecls))
+
+   /\
+
+(* RULE-ID: global-class-definition *)
+(!s0 s name info0 userdefs info edecls.
+     ((info,userdefs) = define_default_specials info0) /\
+     install_member_functions name s0 info.fields s
+   ==>
+     emeaning (Decl (VStrDec name (SOME info0)) :: edecls) s0
+              (copy2globals
+                  (s with <| classmap updated_by
+                                      (\sm. sm |+ (name,
+                                                   SOME (info, userdefs))) |>),
+               edecls))
+`;
+
+
+
